language/move-prover/boogie-backend/src/prelude/native.bpl
@@ -62,27 +62,27 @@ function {:inline} $EmptyVec{{S}}(): Vec ({{T}}) {
     EmptyVec()
 }
 
-procedure {:inline 1} $Vector_empty{{S}}() returns (v: Vec ({{T}})) {
+procedure {:inline 1} $1_Vector_empty{{S}}() returns (v: Vec ({{T}})) {
     v := EmptyVec();
 }
 
-function {:inline} $Vector_$empty{{S}}(): Vec ({{T}}) {
+function {:inline} $1_Vector_$empty{{S}}(): Vec ({{T}}) {
     EmptyVec()
 }
 
-procedure {:inline 1} $Vector_is_empty{{S}}(v: Vec ({{T}})) returns (b: bool) {
+procedure {:inline 1} $1_Vector_is_empty{{S}}(v: Vec ({{T}})) returns (b: bool) {
     b := IsEmptyVec(v);
 }
 
-procedure {:inline 1} $Vector_push_back{{S}}(m: $Mutation (Vec ({{T}})), val: {{T}}) returns (m': $Mutation (Vec ({{T}}))) {
+procedure {:inline 1} $1_Vector_push_back{{S}}(m: $Mutation (Vec ({{T}})), val: {{T}}) returns (m': $Mutation (Vec ({{T}}))) {
     m' := $UpdateMutation(m, ExtendVec($Dereference(m), val));
 }
 
-function {:inline} $Vector_$push_back{{S}}(v: Vec ({{T}}), val: {{T}}): Vec ({{T}}) {
+function {:inline} $1_Vector_$push_back{{S}}(v: Vec ({{T}}), val: {{T}}): Vec ({{T}}) {
     ExtendVec(v, val)
 }
 
-procedure {:inline 1} $Vector_pop_back{{S}}(m: $Mutation (Vec ({{T}}))) returns (e: {{T}}, m': $Mutation (Vec ({{T}}))) {
+procedure {:inline 1} $1_Vector_pop_back{{S}}(m: $Mutation (Vec ({{T}}))) returns (e: {{T}}, m': $Mutation (Vec ({{T}}))) {
     var v: Vec ({{T}});
     var len: int;
     v := $Dereference(m);
@@ -95,23 +95,23 @@ procedure {:inline 1} $Vector_pop_back{{S}}(m: $Mutation (Vec ({{T}}))) returns 
     m' := $UpdateMutation(m, RemoveVec(v));
 }
 
-procedure {:inline 1} $Vector_append{{S}}(m: $Mutation (Vec ({{T}})), other: Vec ({{T}})) returns (m': $Mutation (Vec ({{T}}))) {
+procedure {:inline 1} $1_Vector_append{{S}}(m: $Mutation (Vec ({{T}})), other: Vec ({{T}})) returns (m': $Mutation (Vec ({{T}}))) {
     m' := $UpdateMutation(m, ConcatVec($Dereference(m), other));
 }
 
-procedure {:inline 1} $Vector_reverse{{S}}(m: $Mutation (Vec ({{T}}))) returns (m': $Mutation (Vec ({{T}}))) {
+procedure {:inline 1} $1_Vector_reverse{{S}}(m: $Mutation (Vec ({{T}}))) returns (m': $Mutation (Vec ({{T}}))) {
     m' := $UpdateMutation(m, ReverseVec($Dereference(m)));
 }
 
-procedure {:inline 1} $Vector_length{{S}}(v: Vec ({{T}})) returns (l: int) {
+procedure {:inline 1} $1_Vector_length{{S}}(v: Vec ({{T}})) returns (l: int) {
     l := LenVec(v);
 }
 
-function {:inline} $Vector_$length{{S}}(v: Vec ({{T}})): int {
+function {:inline} $1_Vector_$length{{S}}(v: Vec ({{T}})): int {
     LenVec(v)
 }
 
-procedure {:inline 1} $Vector_borrow{{S}}(v: Vec ({{T}}), i: int) returns (dst: {{T}}) {
+procedure {:inline 1} $1_Vector_borrow{{S}}(v: Vec ({{T}}), i: int) returns (dst: {{T}}) {
     if (!InRangeVec(v, i)) {
         call $ExecFailureAbort();
         return;
@@ -119,11 +119,11 @@ procedure {:inline 1} $Vector_borrow{{S}}(v: Vec ({{T}}), i: int) returns (dst: 
     dst := ReadVec(v, i);
 }
 
-function {:inline} $Vector_$borrow{{S}}(v: Vec ({{T}}), i: int): {{T}} {
+function {:inline} $1_Vector_$borrow{{S}}(v: Vec ({{T}}), i: int): {{T}} {
     ReadVec(v, i)
 }
 
-procedure {:inline 1} $Vector_borrow_mut{{S}}(m: $Mutation (Vec ({{T}})), index: int)
+procedure {:inline 1} $1_Vector_borrow_mut{{S}}(m: $Mutation (Vec ({{T}})), index: int)
 returns (dst: $Mutation ({{T}}), m': $Mutation (Vec ({{T}})))
 {
     var v: Vec ({{T}});
@@ -136,17 +136,17 @@ returns (dst: $Mutation ({{T}}), m': $Mutation (Vec ({{T}})))
     m' := m;
 }
 
-function {:inline} $Vector_$borrow_mut{{S}}(v: Vec ({{T}}), i: int): {{T}} {
+function {:inline} $1_Vector_$borrow_mut{{S}}(v: Vec ({{T}}), i: int): {{T}} {
     ReadVec(v, i)
 }
 
-procedure {:inline 1} $Vector_destroy_empty{{S}}(v: Vec ({{T}})) {
+procedure {:inline 1} $1_Vector_destroy_empty{{S}}(v: Vec ({{T}})) {
     if (!IsEmptyVec(v)) {
       call $ExecFailureAbort();
     }
 }
 
-procedure {:inline 1} $Vector_swap{{S}}(m: $Mutation (Vec ({{T}})), i: int, j: int) returns (m': $Mutation (Vec ({{T}})))
+procedure {:inline 1} $1_Vector_swap{{S}}(m: $Mutation (Vec ({{T}})), i: int, j: int) returns (m': $Mutation (Vec ({{T}})))
 {
     var v: Vec ({{T}});
     v := $Dereference(m);
@@ -157,11 +157,11 @@ procedure {:inline 1} $Vector_swap{{S}}(m: $Mutation (Vec ({{T}})), i: int, j: i
     m' := $UpdateMutation(m, SwapVec(v, i, j));
 }
 
-function {:inline} $Vector_$swap{{S}}(v: Vec ({{T}}), i: int, j: int): Vec ({{T}}) {
+function {:inline} $1_Vector_$swap{{S}}(v: Vec ({{T}}), i: int, j: int): Vec ({{T}}) {
     SwapVec(v, i, j)
 }
 
-procedure {:inline 1} $Vector_remove{{S}}(m: $Mutation (Vec ({{T}})), i: int) returns (e: {{T}}, m': $Mutation (Vec ({{T}})))
+procedure {:inline 1} $1_Vector_remove{{S}}(m: $Mutation (Vec ({{T}})), i: int) returns (e: {{T}}, m': $Mutation (Vec ({{T}})))
 {
     var v: Vec ({{T}});
 
@@ -175,7 +175,7 @@ procedure {:inline 1} $Vector_remove{{S}}(m: $Mutation (Vec ({{T}})), i: int) re
     m' := $UpdateMutation(m, RemoveAtVec(v, i));
 }
 
-procedure {:inline 1} $Vector_swap_remove{{S}}(m: $Mutation (Vec ({{T}})), i: int) returns (e: {{T}}, m': $Mutation (Vec ({{T}})))
+procedure {:inline 1} $1_Vector_swap_remove{{S}}(m: $Mutation (Vec ({{T}})), i: int) returns (e: {{T}}, m': $Mutation (Vec ({{T}})))
 {
     var len: int;
     var v: Vec ({{T}});
@@ -190,12 +190,12 @@ procedure {:inline 1} $Vector_swap_remove{{S}}(m: $Mutation (Vec ({{T}})), i: in
     m' := $UpdateMutation(m, RemoveVec(SwapVec(v, i, len-1)));
 }
 
-procedure {:inline 1} $Vector_contains{{S}}(v: Vec ({{T}}), e: {{T}}) returns (res: bool)  {
+procedure {:inline 1} $1_Vector_contains{{S}}(v: Vec ({{T}}), e: {{T}}) returns (res: bool)  {
     res := $ContainsVec{{S}}(v, e);
 }
 
 procedure {:inline 1}
-$Vector_index_of{{S}}(v: Vec ({{T}}), e: {{T}}) returns (res1: bool, res2: int) {
+$1_Vector_index_of{{S}}(v: Vec ({{T}}), e: {{T}}) returns (res1: bool, res2: int) {
     res2 := $IndexOfVec{{S}}(v, e);
     if (res2 >= 0) {
         res1 := true;
@@ -217,34 +217,34 @@ $Vector_index_of{{S}}(v: Vec ({{T}}), e: {{T}}) returns (res1: bool, res2: int) 
 // Serialize is modeled as an uninterpreted function, with an additional
 // axiom to say it's an injection.
 
-function {:inline} $BCS_serialize{{S}}(v: {{T}}): Vec int;
+function {:inline} $1_BCS_serialize{{S}}(v: {{T}}): Vec int;
 
-axiom (forall v1, v2: {{T}} :: {$BCS_serialize{{S}}(v1), $BCS_serialize{{S}}(v2)}
-   $IsEqual{{S}}(v1, v2) <==> $IsEqual'vec'u8''($BCS_serialize{{S}}(v1), $BCS_serialize{{S}}(v2)));
+axiom (forall v1, v2: {{T}} :: {$1_BCS_serialize{{S}}(v1), $1_BCS_serialize{{S}}(v2)}
+   $IsEqual{{S}}(v1, v2) <==> $IsEqual'vec'u8''($1_BCS_serialize{{S}}(v1), $1_BCS_serialize{{S}}(v2)));
 
 // This says that serialize returns a non-empty vec<u8>
 {% if options.serialize_bound == 0 %}
-axiom (forall v: {{T}} :: {$BCS_serialize{{S}}(v)}
-     ( var r := $BCS_serialize{{S}}(v); $IsValid'vec'u8''(r) && LenVec(r) > 0 ));
+axiom (forall v: {{T}} :: {$1_BCS_serialize{{S}}(v)}
+     ( var r := $1_BCS_serialize{{S}}(v); $IsValid'vec'u8''(r) && LenVec(r) > 0 ));
 {% else %}
-axiom (forall v: {{T}} :: {$BCS_serialize{{S}}(v)}
-     ( var r := $BCS_serialize{{S}}(v); $IsValid'vec'u8''(r) && LenVec(r) > 0 &&
+axiom (forall v: {{T}} :: {$1_BCS_serialize{{S}}(v)}
+     ( var r := $1_BCS_serialize{{S}}(v); $IsValid'vec'u8''(r) && LenVec(r) > 0 &&
                             LenVec(r) <= {{options.serialize_bound}} ));
 {% endif %}
 
-procedure $BCS_to_bytes{{S}}(v: {{T}}) returns (res: Vec int);
-ensures res == $BCS_serialize{{S}}(v);
+procedure $1_BCS_to_bytes{{S}}(v: {{T}}) returns (res: Vec int);
+ensures res == $1_BCS_serialize{{S}}(v);
 
-function {:inline} $BCS_$to_bytes{{S}}(v: {{T}}): Vec int {
-    $BCS_serialize{{S}}(v)
+function {:inline} $1_BCS_$to_bytes{{S}}(v: {{T}}): Vec int {
+    $1_BCS_serialize{{S}}(v)
 }
 
 {% if S == "'address'" -%}
 // Serialized addresses should have the same length.
 const $serialized_address_len: int;
 // Serialized addresses should have the same length
-axiom (forall v: int :: {$BCS_serialize'address'(v)}
-     ( var r := $BCS_serialize'address'(v); LenVec(r) == $serialized_address_len));
+axiom (forall v: int :: {$1_BCS_serialize'address'(v)}
+     ( var r := $1_BCS_serialize'address'(v); LenVec(r) == $serialized_address_len));
 {% endif %}
 {% endmacro hash_module %}
 
@@ -258,13 +258,13 @@ axiom (forall v: int :: {$BCS_serialize'address'(v)}
 {%- set T = instance.name -%}
 
 // Map type specific handle to universal one.
-type $Event_EventHandle{{S}} = $Event_EventHandle;
+type $1_Event_EventHandle{{S}} = $1_Event_EventHandle;
 
-function {:inline} $IsEqual'$Event_EventHandle{{S}}'(a: $Event_EventHandle{{S}}, b: $Event_EventHandle{{S}}): bool {
+function {:inline} $IsEqual'$1_Event_EventHandle{{S}}'(a: $1_Event_EventHandle{{S}}, b: $1_Event_EventHandle{{S}}): bool {
     a == b
 }
 
-function $IsValid'$Event_EventHandle{{S}}'(h: $Event_EventHandle{{S}}): bool {
+function $IsValid'$1_Event_EventHandle{{S}}'(h: $1_Event_EventHandle{{S}}): bool {
     true
 }
 
@@ -276,33 +276,33 @@ axiom (forall v1, v2: {{T}} :: {$ToEventRep{{S}}(v1), $ToEventRep{{S}}(v2)}
 // Creates a new event handle. This ensures each time it is called that a unique new abstract event handler is
 // returned.
 // TODO: we should check (and abort with the right code) if no generator exists for the signer.
-procedure {:inline 1} $Event_new_event_handle{{S}}(signer: int) returns (res: $Event_EventHandle{{S}}) {
-    assume $Event_EventHandles[res] == false;
-    $Event_EventHandles := $Event_EventHandles[res := true];
+procedure {:inline 1} $1_Event_new_event_handle{{S}}(signer: int) returns (res: $1_Event_EventHandle{{S}}) {
+    assume $1_Event_EventHandles[res] == false;
+    $1_Event_EventHandles := $1_Event_EventHandles[res := true];
 }
 
 // This boogie procedure is the model of `emit_event`. This model abstracts away the `counter` behavior, thus not
 // mutating (or increasing) `counter`.
-procedure {:inline 1} $Event_emit_event{{S}}(handle_mut: $Mutation $Event_EventHandle{{S}}, msg: {{T}})
-returns (res: $Mutation $Event_EventHandle{{S}}) {
-    var handle: $Event_EventHandle{{S}};
+procedure {:inline 1} $1_Event_emit_event{{S}}(handle_mut: $Mutation $1_Event_EventHandle{{S}}, msg: {{T}})
+returns (res: $Mutation $1_Event_EventHandle{{S}}) {
+    var handle: $1_Event_EventHandle{{S}};
     handle := $Dereference(handle_mut);
     $es := $ExtendEventStore{{S}}($es, handle, msg);
     res := handle_mut;
 }
 
-procedure {:inline 1} $Event_destroy_handle{{S}}(handle: $Event_EventHandle{{S}}) {
+procedure {:inline 1} $1_Event_destroy_handle{{S}}(handle: $1_Event_EventHandle{{S}}) {
 }
 
 function {:inline} $ExtendEventStore{{S}}(
-        es: $EventStore, handle: $Event_EventHandle{{S}}, msg: {{T}}): $EventStore {
+        es: $EventStore, handle: $1_Event_EventHandle{{S}}, msg: {{T}}): $EventStore {
     (var stream := streams#$EventStore(es)[handle];
     (var stream_new := ExtendMultiset(stream, $ToEventRep{{S}}(msg));
     $EventStore(counter#$EventStore(es)+1, streams#$EventStore(es)[handle := stream_new])))
 }
 
 function {:inline} $CondExtendEventStore{{S}}(
-        es: $EventStore, handle: $Event_EventHandle{{S}}, msg: {{T}}, cond: bool): $EventStore {
+        es: $EventStore, handle: $1_Event_EventHandle{{S}}, msg: {{T}}, cond: bool): $EventStore {
     if cond then
         $ExtendEventStore{{S}}(es, handle, msg)
     else
